PulseHashTable: check for overflow and return bool indicating success. DPE: match on success of hash table operations. BoundedIntegers: add instance for pos.

pulse/share/steel/examples/pulse/dice/dpe/DPE2.fst
@@ -29,8 +29,8 @@ open DPE
   DeriveChild: Part of DPE API 
   Execute the DICE layer associated with the current context and produce a 
   new context. Destroy the current context in the current session's context table 
-  and store the new context in the table.
-  NOTE: Returns 0 upon error
+  and store the new context in the table. Return the new context handle upon
+  success and 0 upon failure. 
 *)
 ```pulse
 fn derive_child (sid:nat) (ctxt_hndl:nat) (record:record_t) (repr:repr_t)
@@ -47,234 +47,282 @@ fn derive_child (sid:nat) (ctxt_hndl:nat) (record:record_t) (repr:repr_t)
   unfold (ht_perm sht_sig sht);
   with spht. assert (models sht_sig sht spht);
 
-  let opt_locked_cht = PHT.lookup #sht_sig #spht sht sid;
+  let res = PHT.lookup #sht_sig #spht sht sid;
+  if (fst res) {
+    let opt_locked_cht = snd res;
+    match opt_locked_cht {
+    Some locked_cht -> {
+      let cht = dfst locked_cht;
+      let cht_lk = dsnd locked_cht;
+      W.acquire #(ht_perm cht_sig cht) cht_lk;
 
-  match opt_locked_cht {
-  Some locked_cht -> {
-    let cht = dfst locked_cht;
-    let cht_lk = dsnd locked_cht;
-    W.acquire #(ht_perm cht_sig cht) cht_lk;
+      unfold (ht_perm cht_sig cht);
+      with cpht. assert (models cht_sig cht cpht);
 
-    unfold (ht_perm cht_sig cht);
-    with cpht0. assert (models cht_sig cht cpht0);
+      let r = PHT.lookup #cht_sig #cpht cht ctxt_hndl;
+      if (fst r) {
+        let opt_locked_ctxt = snd r;
+        match opt_locked_ctxt {
+        Some locked_ctxt -> {
+        let ctxt = dfst locked_ctxt;
+        let ctxt_lk = dsnd locked_ctxt;
+        W.acquire #(context_perm ctxt) ctxt_lk;
 
-    let opt_locked_ctxt = PHT.lookup #cht_sig #cpht0 cht ctxt_hndl;
+        match ctxt {
+        Engine_context c -> {
+          // NOTE: we won't eventually release engine_context_perm because we won't 
+          // own it anymore -- we will disable the uds and free the uds array
+          rewrite (context_perm ctxt) as (engine_context_perm c);
+          unfold (engine_context_perm c);
 
-    match opt_locked_ctxt {
-    Some locked_ctxt -> {
-    let ctxt = dfst locked_ctxt;
-    let ctxt_lk = dsnd locked_ctxt;
-    W.acquire #(context_perm ctxt) ctxt_lk;
+          match record {
+          Engine_record r -> {
+            match repr {
+            Engine_repr r0 -> {       
+              rewrite (record_perm record repr) as (engine_record_perm r r0); 
 
-    match ctxt {
-    Engine_context c -> {
-      // NOTE: we won't eventually release engine_context_perm because we won't 
-      // own it anymore -- we will disable the uds and free the uds array
-      rewrite (context_perm ctxt) as (engine_context_perm c);
-      unfold (engine_context_perm c);
+              let cdi = new_array 0uy dice_digest_len;
+              let ret = EngineCore.engine_main cdi c.uds r;
+              with s. assert (A.pts_to cdi full_perm s);
+              free_array c.uds;
 
-      match record {
-      Engine_record r -> {
-        match repr {
-        Engine_repr r0 -> {       
-          rewrite (record_perm record repr) as (engine_record_perm r r0); 
+              match ret {
+              DICE_SUCCESS -> {
+                let new_locked_context = init_l0_ctxt cdi;
+                free_array cdi #(coerce dice_digest_len s);
+                
+                let d = PHT.delete #cht_sig #cpht cht ctxt_hndl;
+                if d {
+                  assert (models cht_sig cht (LSHT.delete cpht ctxt_hndl));
+                  let b = not_full #cht_sig #(LSHT.delete cpht ctxt_hndl) cht;
+                  if b {
+                    let i = PHT.insert #cht_sig #(LSHT.delete cpht ctxt_hndl) cht new_ctxt_hndl new_locked_context; 
+                    if i {
+                      assert (models cht_sig cht (LSHT.insert (LSHT.delete cpht ctxt_hndl) new_ctxt_hndl new_locked_context));
+                      rewrite (engine_record_perm r r0) as (record_perm record repr);
+                      fold (ht_perm sht_sig sht);
+                      fold (ht_perm cht_sig cht);
+                      W.release #(ht_perm sht_sig sht) sht_lk;
+                      W.release #(ht_perm cht_sig cht) cht_lk;
+                      new_ctxt_hndl
+                    } else {
+                      // ERROR - insert failed
+                      assert (models cht_sig cht (LSHT.delete cpht ctxt_hndl));
+                      rewrite (engine_record_perm r r0) as (record_perm record repr);
+                      fold (ht_perm sht_sig sht);
+                      fold (ht_perm cht_sig cht);
+                      W.release #(ht_perm sht_sig sht) sht_lk;
+                      W.release #(ht_perm cht_sig cht) cht_lk;
+                      0
+                  }} else {
+                    // ERROR -- table full
+                    rewrite (engine_record_perm r r0) as (record_perm record repr);
+                    fold (ht_perm sht_sig sht);
+                    fold (ht_perm cht_sig cht);
+                    W.release #(ht_perm sht_sig sht) sht_lk;
+                    W.release #(ht_perm cht_sig cht) cht_lk;
+                    0
+                }} else {
+                  // ERROR - delete failed
+                  assert (models cht_sig cht cpht);
+                  rewrite (engine_record_perm r r0) as (record_perm record repr);
+                  fold (ht_perm sht_sig sht);
+                  fold (ht_perm cht_sig cht);
+                  W.release #(ht_perm sht_sig sht) sht_lk;
+                  W.release #(ht_perm cht_sig cht) cht_lk;
+                  0
+                }}
+              DICE_ERROR -> {
+                // ERROR -- DICE engine failed
+                free_array cdi #(coerce dice_digest_len s);
+                rewrite (engine_record_perm r r0) as (record_perm record repr);
+                fold (ht_perm sht_sig sht);
+                fold (ht_perm cht_sig cht);
+                W.release #(ht_perm sht_sig sht) sht_lk;
+                W.release #(ht_perm cht_sig cht) cht_lk;
+                0
+              }}}
+            _ -> {
+              // ERROR - repr should have type (Egnine_repr r0)
+              zeroize_array uds_len c.uds #uds_bytes;
+              disable_uds ();
+              free_array c.uds;
 
-          let cdi = new_array 0uy dice_digest_len;
-          let ret = EngineCore.engine_main cdi c.uds r;
-          with s. assert (A.pts_to cdi full_perm s);
-          free_array c.uds;
-
-          match ret {
-          DICE_SUCCESS -> {
-            let new_locked_context = init_l0_ctxt cdi;
-            free_array cdi #(coerce dice_digest_len s);
-            
-            PHT.delete #cht_sig #cpht0 cht ctxt_hndl;
-            with cpht1. assert (models cht_sig cht cpht1);
-            let b = not_full #cht_sig #cpht1 cht;
-
-            if b {
-              PHT.insert #cht_sig #cpht1 cht new_ctxt_hndl new_locked_context; 
-
-              rewrite (engine_record_perm r r0) as (record_perm record repr);
               fold (ht_perm sht_sig sht);
               fold (ht_perm cht_sig cht);
               W.release #(ht_perm sht_sig sht) sht_lk;
               W.release #(ht_perm cht_sig cht) cht_lk;
+              0
+            }}
+          }
+          _ -> {
+            // ERROR - record should have type (Engine_record r)
+            zeroize_array uds_len c.uds;
+            disable_uds ();
+            free_array c.uds;
 
-              new_ctxt_hndl
-            } else {
-              // ERROR -- table full
-              rewrite (engine_record_perm r r0) as (record_perm record repr);
-              fold (ht_perm sht_sig sht);
-              fold (ht_perm cht_sig cht);
-              W.release #(ht_perm sht_sig sht) sht_lk;
-              W.release #(ht_perm cht_sig cht) cht_lk;
-
-              new_ctxt_hndl
-          }}
-          DICE_ERROR -> {
-            // ERROR -- DICE engine failed
-            free_array cdi #(coerce dice_digest_len s);
-            rewrite (engine_record_perm r r0) as (record_perm record repr);
             fold (ht_perm sht_sig sht);
             fold (ht_perm cht_sig cht);
             W.release #(ht_perm sht_sig sht) sht_lk;
             W.release #(ht_perm cht_sig cht) cht_lk;
             0
-          }}}
-        _ -> {
-          // ERROR - repr should have type (Egnine_repr r0)
-          zeroize_array uds_len c.uds #uds_bytes;
-          disable_uds ();
-          free_array c.uds;
-
-          fold (ht_perm sht_sig sht);
-          fold (ht_perm cht_sig cht);
-          W.release #(ht_perm sht_sig sht) sht_lk;
-          W.release #(ht_perm cht_sig cht) cht_lk;
-          0
-        }}
-      }
-      _ -> {
-        // ERROR - record should have type (Engine_record r)
-        zeroize_array uds_len c.uds;
-        disable_uds ();
-        free_array c.uds;
-
-        fold (ht_perm sht_sig sht);
-        fold (ht_perm cht_sig cht);
-        W.release #(ht_perm sht_sig sht) sht_lk;
-        W.release #(ht_perm cht_sig cht) cht_lk;
-        0
-      }}
-    }
-    L0_context c -> {
-      // NOTE: we won't eventually release l0_context_perm because we won't 
-      // own it anymore -- we will free the cdi array
-      rewrite (context_perm ctxt) as (l0_context_perm c);
-      unfold (l0_context_perm c);
-
-      with s. assert (A.pts_to c.cdi full_perm s);
-
-      match record {
-      L0_record r -> {
-        match repr {
-        L0_repr r0 -> {
-          let idcsr_ing = r.deviceIDCSR_ingredients;
-          let akcrt_ing = r.aliasKeyCRT_ingredients;
-
-          let deviceIDCRI_len = len_of_deviceIDCRI  idcsr_ing.version idcsr_ing.s_common 
-                                                    idcsr_ing.s_org idcsr_ing.s_country;
-          let aliasKeyTBS_len = len_of_aliasKeyTBS  akcrt_ing.serialNumber akcrt_ing.i_common 
-                                                    akcrt_ing.i_org akcrt_ing.i_country 
-                                                    akcrt_ing.s_common akcrt_ing.s_org 
-                                                    akcrt_ing.s_country akcrt_ing.l0_version;
-          let deviceIDCSR_len = length_of_deviceIDCSR deviceIDCRI_len;
-          let aliasKeyCRT_len = length_of_aliasKeyCRT aliasKeyTBS_len;
-
-          let deviceID_pub = new_array 0uy v32us;
-          let deviceID_priv = new_array 0uy v32us;
-          let aliasKey_pub = new_array 0uy v32us;
-          let aliasKey_priv = new_array 0uy v32us;
-          let deviceIDCSR = new_array 0uy deviceIDCSR_len;
-          let aliasKeyCRT = new_array 0uy aliasKeyCRT_len;
-
-          rewrite (record_perm record repr) as (l0_record_perm r r0); 
-
-          assume_ (pure(valid_hkdf_ikm_len (digest_len dice_hash_alg)));
-          
-          L0Core.l0_main  c.cdi deviceID_pub deviceID_priv 
-                          aliasKey_pub aliasKey_priv 
-                          aliasKeyTBS_len aliasKeyCRT_len aliasKeyCRT 
-                          deviceIDCRI_len deviceIDCSR_len deviceIDCSR r;
-          free_array c.cdi;
-
-          with (s1:elseq U8.t v32us). assert (A.pts_to aliasKey_priv full_perm s1);
-          let new_locked_context = init_l1_ctxt deviceIDCSR_len aliasKeyCRT_len 
-                                                deviceID_priv deviceID_pub
-                                                aliasKey_priv aliasKey_pub 
-                                                deviceIDCSR aliasKeyCRT;
-          free_array deviceID_pub;
-          free_array deviceID_priv;
-          free_array aliasKey_pub;
-          free_array aliasKey_priv;
-          free_array deviceIDCSR;
-          free_array aliasKeyCRT;
-          
-          PHT.delete #cht_sig #cpht0 cht ctxt_hndl;
-          with cpht1. assert (models cht_sig cht cpht1);
-          let b = not_full #cht_sig #cpht1 cht;
-
-          if b {
-            PHT.insert #cht_sig #cpht1 cht new_ctxt_hndl new_locked_context;
-
-            rewrite (l0_record_perm r r0) as (record_perm record repr);
-
-            fold (ht_perm sht_sig sht);
-            fold (ht_perm cht_sig cht);
-            W.release #(ht_perm sht_sig sht) sht_lk;
-            W.release #(ht_perm cht_sig cht) cht_lk;
-
-            new_ctxt_hndl
-          } else {
-            // ERROR -- table full
-            rewrite (l0_record_perm r r0) as (record_perm record repr);
-
-            fold (ht_perm sht_sig sht);
-            fold (ht_perm cht_sig cht);
-            W.release #(ht_perm sht_sig sht) sht_lk;
-            W.release #(ht_perm cht_sig cht) cht_lk;
-
-            new_ctxt_hndl
-          }
+          }}
         }
-        _ -> {
-          // ERROR - repr should have type (L0_repr r0)
-          zeroize_array dice_digest_len c.cdi;
-          free_array c.cdi;
+        L0_context c -> {
+          // NOTE: we won't eventually release l0_context_perm because we won't 
+          // own it anymore -- we will free the cdi array
+          rewrite (context_perm ctxt) as (l0_context_perm c);
+          unfold (l0_context_perm c);
 
+          with s. assert (A.pts_to c.cdi full_perm s);
+
+          match record {
+          L0_record r -> {
+            match repr {
+            L0_repr r0 -> {
+              let idcsr_ing = r.deviceIDCSR_ingredients;
+              let akcrt_ing = r.aliasKeyCRT_ingredients;
+
+              let deviceIDCRI_len = len_of_deviceIDCRI  idcsr_ing.version idcsr_ing.s_common 
+                                                        idcsr_ing.s_org idcsr_ing.s_country;
+              let aliasKeyTBS_len = len_of_aliasKeyTBS  akcrt_ing.serialNumber akcrt_ing.i_common 
+                                                        akcrt_ing.i_org akcrt_ing.i_country 
+                                                        akcrt_ing.s_common akcrt_ing.s_org 
+                                                        akcrt_ing.s_country akcrt_ing.l0_version;
+              let deviceIDCSR_len = length_of_deviceIDCSR deviceIDCRI_len;
+              let aliasKeyCRT_len = length_of_aliasKeyCRT aliasKeyTBS_len;
+
+              let deviceID_pub = new_array 0uy v32us;
+              let deviceID_priv = new_array 0uy v32us;
+              let aliasKey_pub = new_array 0uy v32us;
+              let aliasKey_priv = new_array 0uy v32us;
+              let deviceIDCSR = new_array 0uy deviceIDCSR_len;
+              let aliasKeyCRT = new_array 0uy aliasKeyCRT_len;
+
+              rewrite (record_perm record repr) as (l0_record_perm r r0); 
+
+              assume_ (pure(valid_hkdf_ikm_len (digest_len dice_hash_alg)));
+              
+              L0Core.l0_main  c.cdi deviceID_pub deviceID_priv 
+                              aliasKey_pub aliasKey_priv 
+                              aliasKeyTBS_len aliasKeyCRT_len aliasKeyCRT 
+                              deviceIDCRI_len deviceIDCSR_len deviceIDCSR r;
+              free_array c.cdi;
+
+              with (s1:elseq U8.t v32us). assert (A.pts_to aliasKey_priv full_perm s1);
+              let new_locked_context = init_l1_ctxt deviceIDCSR_len aliasKeyCRT_len 
+                                                    deviceID_priv deviceID_pub
+                                                    aliasKey_priv aliasKey_pub 
+                                                    deviceIDCSR aliasKeyCRT;
+              free_array deviceID_pub;
+              free_array deviceID_priv;
+              free_array aliasKey_pub;
+              free_array aliasKey_priv;
+              free_array deviceIDCSR;
+              free_array aliasKeyCRT;
+              
+              let d = PHT.delete #cht_sig #cpht cht ctxt_hndl;
+              if d {
+                assert (models cht_sig cht (LSHT.delete cpht ctxt_hndl));
+                let b = not_full #cht_sig #(LSHT.delete cpht ctxt_hndl) cht;
+                if b {
+                  let i = PHT.insert #cht_sig #(LSHT.delete cpht ctxt_hndl) cht new_ctxt_hndl new_locked_context;
+                  if i {
+                    assert (models cht_sig cht (LSHT.insert (LSHT.delete cpht ctxt_hndl) new_ctxt_hndl new_locked_context));
+                    rewrite (l0_record_perm r r0) as (record_perm record repr);
+                    fold (ht_perm sht_sig sht);
+                    fold (ht_perm cht_sig cht);
+                    W.release #(ht_perm sht_sig sht) sht_lk;
+                    W.release #(ht_perm cht_sig cht) cht_lk;
+                    new_ctxt_hndl
+                  } else {
+                    // ERROR - insert failed
+                    assert (models cht_sig cht (LSHT.delete cpht ctxt_hndl));
+                    rewrite (l0_record_perm r r0) as (record_perm record repr);
+                    fold (ht_perm sht_sig sht);
+                    fold (ht_perm cht_sig cht);
+                    W.release #(ht_perm sht_sig sht) sht_lk;
+                    W.release #(ht_perm cht_sig cht) cht_lk;
+                    0
+                }} else {
+                  // ERROR - table full
+                  rewrite (l0_record_perm r r0) as (record_perm record repr);
+                  fold (ht_perm sht_sig sht);
+                  fold (ht_perm cht_sig cht);
+                  W.release #(ht_perm sht_sig sht) sht_lk;
+                  W.release #(ht_perm cht_sig cht) cht_lk;
+                  0
+              }} else {
+                // ERROR - delete failed
+                assert (models cht_sig cht cpht);
+                rewrite (l0_record_perm r r0) as (record_perm record repr);
+                fold (ht_perm sht_sig sht);
+                fold (ht_perm cht_sig cht);
+                W.release #(ht_perm sht_sig sht) sht_lk;
+                W.release #(ht_perm cht_sig cht) cht_lk;
+                0
+              }
+            }
+            _ -> {
+              // ERROR - repr should have type (L0_repr r0)
+              zeroize_array dice_digest_len c.cdi;
+              free_array c.cdi;
+
+              fold (ht_perm sht_sig sht);
+              fold (ht_perm cht_sig cht);
+              W.release #(ht_perm sht_sig sht) sht_lk;
+              W.release #(ht_perm cht_sig cht) cht_lk;
+              0
+            }}
+          }
+          _ -> {
+            // ERROR - record should have type (L0_record r)
+            zeroize_array dice_digest_len c.cdi;
+            free_array c.cdi;
+
+            fold (ht_perm sht_sig sht);
+            fold (ht_perm cht_sig cht);
+            W.release #(ht_perm sht_sig sht) sht_lk;
+            W.release #(ht_perm cht_sig cht) cht_lk;
+            0
+          }}
+        }
+        _ -> { 
+          // ERROR - cannot invoke DeriveChild with L1 context
           fold (ht_perm sht_sig sht);
           fold (ht_perm cht_sig cht);
+          W.release #(context_perm ctxt) ctxt_lk;
           W.release #(ht_perm sht_sig sht) sht_lk;
           W.release #(ht_perm cht_sig cht) cht_lk;
           0
+        }}}
+        None -> { 
+        // ERROR - bad context handle
+        fold (ht_perm sht_sig sht);
+        fold (ht_perm cht_sig cht);
+        W.release #(ht_perm sht_sig sht) sht_lk;
+        W.release #(ht_perm cht_sig cht) cht_lk;
+        0
         }}
-      }
-      _ -> {
-        // ERROR - record should have type (L0_record r)
-        zeroize_array dice_digest_len c.cdi;
-        free_array c.cdi;
-
+      } else {
+        // ERROR - lookup failed
         fold (ht_perm sht_sig sht);
         fold (ht_perm cht_sig cht);
         W.release #(ht_perm sht_sig sht) sht_lk;
         W.release #(ht_perm cht_sig cht) cht_lk;
         0
       }}
-    }
-    _ -> { 
-      // ERROR - cannot invoke DeriveChild with L1 context
-      fold (ht_perm sht_sig sht);
-      fold (ht_perm cht_sig cht);
-      W.release #(context_perm ctxt) ctxt_lk;
-      W.release #(ht_perm sht_sig sht) sht_lk;
-      W.release #(ht_perm cht_sig cht) cht_lk;
-      0
-    }}}
     None -> { 
-    // ERROR - bad context handle
+    // ERROR - bad session ID
     fold (ht_perm sht_sig sht);
-    fold (ht_perm cht_sig cht);
     W.release #(ht_perm sht_sig sht) sht_lk;
-    W.release #(ht_perm cht_sig cht) cht_lk;
     0
-    }}}
-  None -> { 
-  // ERROR - bad session ID
-  fold (ht_perm sht_sig sht);
-  W.release #(ht_perm sht_sig sht) sht_lk;
-  0
-  }}
+    }}
+  } else {
+    // ERROR - lookup failed
+    fold (ht_perm sht_sig sht);
+    W.release #(ht_perm sht_sig sht) sht_lk;
+    0
+  }
 }
 ```
