pulse/lib/steel/pulse/Pulse.Class.BoundedIntegers.fst
@@ -85,6 +85,20 @@ instance bounded_int_nat : bounded_int nat = {
 let add_nat (x y:nat) = x + y
 //but we should find a way to make it work with refinement, otherwise we'll need instances for pos etc. too
 
+let pos_as_int (x:pos) : int = x
+
+instance bounded_int_pos : bounded_int pos = {
+    fits = (fun x -> x > 0);
+    v = pos_as_int;
+    u = (fun x -> x);
+    ( + ) = (fun x y -> Prims.op_Addition x y);
+    op_Subtraction = (fun x y -> Prims.op_Subtraction x y); //can't write ( - ), it doesn't parse
+    ( < ) = (fun x y -> Prims.op_LessThan x y);
+    ( <= ) = (fun x y -> Prims.op_LessThanOrEqual x y);
+    ( % ) = (fun x y -> Prims.op_Modulus x y);
+    properties = ()
+}
+
 // Using a fits predicate as the bounds check allows this class to also accomodate SizeT
 open FStar.SizeT
 instance bounded_int_size_t : bounded_int FStar.SizeT.t = {
